theories/logic/compatibility.v
@@ -44,144 +44,153 @@ Section compatibility.
   (* Base rules *)
   
   Lemma sem_typed_unit Γ : 
-    ⊢ Γ ⊨ #() : ⟨⟩ : ().
+    ⊢ Γ ⊨ #() : ⟨⟩ : () ⊨ Γ.
   Proof.
-    iIntros (vs) "!# HΓ //=". by iApply ewp_value.
+    iIntros (vs) "!# HΓ₁ //=". iApply ewp_value. by iFrame.
   Qed.
   
   Lemma sem_typed_bool Γ (b : bool) : 
-    ⊢ Γ ⊨ #b : ⟨⟩ : 𝔹.
+    ⊢ Γ ⊨ #b : ⟨⟩ : 𝔹 ⊨ Γ.
   Proof.
-    iIntros (vs) "!# HΓ //=". iApply ewp_value. by iExists b.
+    iIntros (vs) "!# HΓ₁ //=". iApply ewp_value. 
+    iSplitR; first (iExists b); done.
   Qed.
   
   Lemma sem_typed_int Γ (i : Z) : 
-    ⊢ Γ ⊨ #i : ⟨⟩ : ℤ.
+    ⊢ Γ ⊨ #i : ⟨⟩ : ℤ ⊨ Γ.
   Proof.
-    iIntros (vs) "!# HΓ //=". iApply ewp_value. by iExists i.
+    iIntros (vs) "!# HΓ₁ //=". iApply ewp_value. 
+    iSplitR; first (iExists i); done.
   Qed.
   
   (* Subsumption rule *)
   
-  Lemma sem_typed_sub Γ Γ' e ρ ρ' τ τ':
-    Γ ≤E Γ' →
+  Lemma sem_typed_sub Γ₁ Γ₁' Γ₂ Γ₂' e ρ ρ' τ τ':
+    Γ₁  ≤E Γ₁' →
+    Γ₂' ≤E Γ₂ →
     ρ'  ≤R ρ → 
     τ'  ≤T τ →
-    Γ' ⊨ e : ρ' : τ' -∗ Γ ⊨ e : ρ : τ.
+    Γ₁' ⊨ e : ρ' : τ' ⊨ Γ₂' -∗ Γ₁ ⊨ e : ρ : τ ⊨ Γ₂.
   Proof.
-    iIntros (HΓle Hρle Hτle) "#He !# %vs HΓ //=".
-    rewrite HΓle.
+    iIntros (HΓ₁le HΓ₂le Hρle Hτle) "#He !# %vs HΓ₁ //=".
+    rewrite HΓ₁le.
     iApply ewp_os_prot_mono.
     { iApply Hρle. }
-    iApply (ewp_mono with "[HΓ He]").
+    iApply (ewp_mono with "[HΓ₁ He]").
     { by iApply "He". }
-    iIntros (v) "Hτ'". iModIntro.
-    by iApply Hτle.
+    iIntros (v) "(Hτ' & HΓ₂)". iModIntro.
+    rewrite HΓ₂le.
+    iSplitR "HΓ₂"; first (iApply Hτle); done.
   Qed. 
   
   (* λ-calculus rules *)
-  
-  Lemma sem_typed_lfun Γ x e τ ρ κ: 
-    x ∉ (env_dom Γ) →
-    (x,τ) :: Γ ⊨ e : ρ : κ -∗
-    Γ ⊨ (λ: x, e) : ⟨⟩ : (τ -{ ρ }-∘ κ).
+
+  Lemma sem_typed_afun Γ₁ Γ₂ x e τ ρ κ: 
+    x ∉ (env_dom Γ₁) →
+    x ∉ (env_dom Γ₂) →
+    (x,τ) :: Γ₁ ⊨ e : ρ : κ ⊨ [] -∗
+    Γ₁ ++ Γ₂ ⊨ (λ: x, e) : ⟨⟩ : (τ -{ ρ }-∘ κ) ⊨ Γ₂.
   Proof.
-    iIntros (Helem) "#He !# %vs HΓ //=".
-    ewp_pure_steps. iIntros (w) "Hw". ewp_pure_steps. 
-    rewrite <- subst_map_insert.
-    iApply "He". simpl in *. iSplitL "Hw".
-    - iExists w. iFrame. iPureIntro.
-      by rewrite lookup_insert.
-    - by iApply env_sem_typed_insert.
+    iIntros (??) "#He !# %vs HΓ₁₂ //=".
+    ewp_pure_steps. 
+    rewrite env_sem_typed_app. iDestruct "HΓ₁₂" as "[HΓ₁ $]".
+    iIntros (w) "Hτ". ewp_pure_steps.
+    rewrite -subst_map_insert. 
+    iApply (ewp_mono with "[HΓ₁ Hτ]").
+    - iApply "He". simpl. 
+      iSplitL "Hτ". 
+      { iExists w. iFrame. iPureIntro. apply lookup_insert. }
+      by iApply env_sem_typed_insert.
+    - iIntros (v) "//= [Hκ _] !> {$Hκ}". 
   Qed.
   
-  Lemma sem_typed_ufun Γ f x e τ ρ κ: 
-    x ∉ (env_dom Γ) →
-    f ∉ (env_dom Γ) →
+  Lemma sem_typed_ufun Γ₁ Γ₂ f x e τ ρ κ: 
+    x ∉ (env_dom Γ₁) →
+    f ∉ (env_dom Γ₁) →
     x ≠ f →
-    copy_env Γ →
-    (x,τ) :: (f, τ -{ ρ }-> κ) :: Γ ⊨ e : ρ : κ -∗
-    Γ ⊨ (rec: f x := e) : ⟨⟩ : (τ -{ ρ }-> κ).
+    copy_env Γ₁ →
+    (x,τ) :: (f, τ -{ ρ }-> κ) :: Γ₁ ⊨ e : ρ : κ ⊨ [] -∗
+    Γ₁ ++ Γ₂ ⊨ (rec: f x := e) : ⟨⟩ : (τ -{ ρ }-> κ) ⊨ Γ₂.
   Proof.
-    iIntros (Helemx Helemf Hneq HcpyΓ) "#He !# %vs HΓ //=".
-    ewp_pure_steps. rewrite HcpyΓ. iDestruct "HΓ" as "#HΓ".
+    iIntros (??? HcpyΓ₁) "#He !# %vs HΓ₁₂ //=".
+    ewp_pure_steps.
+    rewrite env_sem_typed_app. iDestruct "HΓ₁₂" as "[HΓ₁ $]".
+    rewrite HcpyΓ₁. iDestruct "HΓ₁" as "#HΓ₁".
     iLöb as "IH".
     iIntros (w) "!# Hw". ewp_pure_steps. 
     rewrite subst_subst_ne; last done.
     rewrite -subst_map_insert.
     rewrite -delete_insert_ne; last done. 
     rewrite -subst_map_insert.
-    iApply "He". simpl in *. iSplitL "Hw"; last iSplitR "HΓ".
-    - iExists w. iFrame. iPureIntro.
-      rewrite lookup_insert_ne; last done.
-      by rewrite lookup_insert.
-    - iExists _. iSplit; [by rewrite lookup_insert|]. 
-      iApply "IH".
-    - by do 2 (iApply env_sem_typed_insert; first done).
+    iApply (ewp_mono with "[He Hw]").
+    - iApply "He". simpl in *. iSplitL "Hw"; last iSplitR "HΓ₁".
+      + iExists w. iFrame. iPureIntro.
+        rewrite lookup_insert_ne; last done.
+        by rewrite lookup_insert.
+      + iExists _. iSplit; [by rewrite lookup_insert|]. 
+        iApply "IH".
+      + by do 2 (iApply env_sem_typed_insert; first done).
+    - iIntros (v) "(Hκ & _) !> {$Hκ}".
   Qed.
   
-  Lemma sem_typed_app Γ₁ Γ₂ e₁ e₂ τ ρ κ: 
-    Γ₁ ⊨ e₁ : ρ : (τ -{ ρ }-∘ κ) -∗
-    Γ₂ ⊨ e₂ : ρ : τ -∗
-    Γ₁ ++ Γ₂ ⊨ (e₁ e₂) : ρ : κ.
+  Lemma sem_typed_app Γ₁ Γ₂ Γ₃ e₁ e₂ τ ρ κ: 
+    Γ₂ ⊨ e₁ : ρ : (τ -{ ρ }-∘ κ) ⊨ Γ₃ -∗
+    Γ₁ ⊨ e₂ : ρ : τ ⊨ Γ₂ -∗
+    Γ₁ ⊨ (e₁ e₂) : ρ : κ ⊨ Γ₃.
   Proof.
-    iIntros "#He₁ #He₂ !# %vs HΓ₁₂ //=".
-    rewrite env_sem_typed_app.
-    iDestruct "HΓ₁₂" as "[HΓ₁ HΓ₂]".
+    iIntros "#He₁ #He₂ !# %vs HΓ₁ //=".
     iApply (ewp_bind ([AppRCtx (subst_map vs e₁)])); first done.
-    iApply (ewp_mono with "[HΓ₂]").
+    iApply (ewp_mono with "[HΓ₁]").
     { by iApply "He₂". }
-    iIntros (v) "Hτv //=". iModIntro.
+    iIntros (v) "[Hτv HΓ₂] //= !>".
     iApply (ewp_bind ([AppLCtx v])); first done.
-    iApply (ewp_mono with "[HΓ₁]").
-    { by iApply "He₁". }
-    iIntros (w) "Hτκw //=". iModIntro; by iApply "Hτκw". 
-  Qed.
-  
-  Lemma sem_typed_pair Γ₁ Γ₂ e₁ e₂ τ ρ κ: 
-    Γ₁ ⊨ e₁ : ρ : τ -∗
-    Γ₂ ⊨ e₂ : ρ : κ -∗
-    Γ₁ ++ Γ₂ ⊨ (e₁,e₂) : ρ : (τ × κ).
-  Proof.
-    iIntros "#He₁ #He₂ !# %vs HΓ₁₂ //=".
-    rewrite env_sem_typed_app.
-    iDestruct "HΓ₁₂" as "[HΓ₁ HΓ₂]".
-    iApply (ewp_bind ([PairRCtx (subst_map vs e₁)])); first done.
     iApply (ewp_mono with "[HΓ₂]").
-    { by iApply "He₂". }
-    iIntros (v) "Hτv //=". iModIntro.
-    iApply (ewp_bind ([PairLCtx v])); first done.
-    iApply (ewp_mono with "[HΓ₁]").
     { by iApply "He₁". }
-    iIntros (w) "Hκw //=". iModIntro. ewp_pure_steps.
-    iExists w, v. iFrame. by iPureIntro.
+    iIntros (w) "[Hτκw HΓ₃] //= !>". 
+    iApply (ewp_frame_r with "[Hτκw Hτv] HΓ₃").
+    by iApply "Hτκw".
   Qed.
   
-  Lemma sem_typed_pair_elim Γ₁ Γ₂ x₁ x₂ e₁ e₂ τ ρ κ ι: 
-    x₁ ∉ (env_dom Γ₂) ->
-    x₂ ∉ (env_dom Γ₂) ->
-    x₁ ≠ x₂ ->
-    Γ₁ ⊨ e₁ : ρ : (τ × κ) -∗
-    (x₁, τ) :: (x₂, κ) :: Γ₂ ⊨ e₂ : ρ : ι -∗
-    Γ₁ ++ Γ₂ ⊨ (let: (x₁, x₂) := e₁ in e₂) : ρ : ι.
+  Lemma sem_typed_pair Γ₁ Γ₂ Γ₃ e₁ e₂ τ ρ κ: 
+    Γ₂ ⊨ e₁ : ρ : τ ⊨ Γ₃ -∗
+    Γ₁ ⊨ e₂ : ρ : κ ⊨ Γ₂ -∗
+    Γ₁ ⊨ (e₁,e₂) : ρ : (τ × κ) ⊨ Γ₃.
   Proof.
-    iIntros (Helem₁ Helem₂ Hnex₁₂) "#He₁ #He₂ !# %vs HΓ₁₂ //=".
-    rewrite env_sem_typed_app.
-    iDestruct "HΓ₁₂" as "[HΓ₁ HΓ₂]".
+    iIntros "#He₁ #He₂ !# %vs HΓ₁ //=".
+    iApply (ewp_bind ([PairRCtx (subst_map vs e₁)])); first done.
+    iApply (ewp_mono with "[HΓ₁]").
+    { by iApply "He₂". }
+    iIntros (v) "[Hτv HΓ₂] //= !>".
+    iApply (ewp_bind ([PairLCtx v])); first done.
+    iApply (ewp_mono with "[HΓ₂]").
+    { by iApply "He₁". }
+    iIntros (w) "[Hκw HΓ₃] //= !> ". ewp_pure_steps.
+    iFrame. iExists w, v. iFrame. by iPureIntro.
+  Qed.
+  
+  Lemma sem_typed_pair_elim Γ₁ Γ₂ Γ₃ x₁ x₂ e₁ e₂ τ ρ κ ι: 
+    x₁ ∉ (env_dom Γ₂) → x₂ ∉ (env_dom Γ₂) →
+    x₁ ∉ (env_dom Γ₃) → x₂ ∉ (env_dom Γ₃) →
+    x₁ ≠ x₂ →
+    Γ₁ ⊨ e₁ : ρ : (τ × κ) ⊨ Γ₂ -∗
+    (x₁, τ) :: (x₂, κ) :: Γ₂ ⊨ e₂ : ρ : ι ⊨ Γ₃ -∗
+    Γ₁ ⊨ (let: (x₁, x₂) := e₁ in e₂) : ρ : ι ⊨ Γ₃.
+  Proof.
+    iIntros (?????) "#He₁ #He₂ !# %vs HΓ₁ //=".
     ewp_pure_steps.
     set ex1x2 := (λ: x₁ x₂, subst_map (binder_delete x₂ 
                                       (binder_delete x₁ vs)) e₂)%V. 
     iApply (ewp_bind ([AppLCtx ex1x2; AppRCtx pair_elim])); first done.
     iApply (ewp_mono with "[HΓ₁]").
     { by iApply "He₁". }
-    iIntros (v) "Hτκv". iModIntro. simpl in *. 
+    iIntros (v) "[Hτκv HΓ₂] !> //=". 
     unfold pair_elim. ewp_pure_steps.
     iDestruct "Hτκv" as "(%v₁ & %v₂ & -> & Hτ & Hκ)".
     unfold ex1x2. ewp_pure_steps. 
     destruct (decide _) as [[]|[]]; [|split; [done|congruence]].
-    rewrite delete_commute -subst_map_insert -delete_insert_ne
-      ;last congruence.
+    rewrite delete_commute -subst_map_insert -delete_insert_ne; last congruence.
     rewrite <- subst_map_insert.
+    iApply (ewp_mono with "[Hτ Hκ HΓ₂]"). 
     iApply "He₂". simpl. iSplitL "Hτ".
     { iExists v₁. iFrame. iPureIntro. 
       rewrite lookup_insert_ne; last done.
@@ -190,192 +199,193 @@ Section compatibility.
     { iExists v₂. iFrame. iPureIntro. 
       by rewrite lookup_insert. }
     by repeat (iApply env_sem_typed_insert; first done).
+    iIntros (v) "[Hιv HΓ₃] !> {$Hιv}".
+    iApply (env_sem_typed_delete _ _ x₁ v₁); first done.
+    iApply (env_sem_typed_delete _ _ x₂ v₂); done.
   Qed.
   
-  Lemma sem_typed_un_op Γ e op τ κ ρ: 
+  Lemma sem_typed_un_op Γ₁ Γ₂ e op τ κ ρ: 
     typed_un_op op τ κ →
-    Γ ⊨ e : ρ : τ -∗
-    Γ ⊨ UnOp op e : ρ : κ.
+    Γ₁ ⊨ e : ρ : τ ⊨ Γ₂-∗
+    Γ₁ ⊨ UnOp op e : ρ : κ ⊨ Γ₂.
   Proof.
-    iIntros (Hop) "#He !# %vs HΓ //=".
+    iIntros (Hop) "#He !# %vs HΓ₁ //=".
     iApply (ewp_bind [UnOpCtx _]); first done.
-    iApply (ewp_mono with "[HΓ]").
+    iApply (ewp_mono with "[HΓ₁]").
     { by iApply "He". }
-    iIntros (v) "Hv !> //=".
+    iIntros (v) "[Hv HΓ₂] !> //=".
     destruct op; inversion_clear Hop;
     iDestruct "Hv" as "(%n & ->)";
     ewp_pure_steps; eauto.
   Qed.
   
-  Lemma sem_typed_bin_op Γ₁ Γ₂ e₁ e₂ op τ κ ι ρ: 
+  Lemma sem_typed_bin_op Γ₁ Γ₂ Γ₃ e₁ e₂ op τ κ ι ρ: 
     typed_bin_op op τ κ ι →
-    Γ₁ ⊨ e₁ : ρ : τ -∗
-    Γ₂ ⊨ e₂ : ρ : κ -∗
-    Γ₁ ++ Γ₂ ⊨ BinOp op e₁ e₂ : ρ : ι.
+    Γ₂ ⊨ e₁ : ρ : τ ⊨ Γ₃ -∗
+    Γ₁ ⊨ e₂ : ρ : κ ⊨ Γ₂ -∗
+    Γ₁ ⊨ BinOp op e₁ e₂ : ρ : ι ⊨ Γ₃.
   Proof.
-    iIntros (Hop) "#He₁ #He₂ !# %vs HΓ₁₂ //=".
-    rewrite env_sem_typed_app.
-    iDestruct "HΓ₁₂" as "[HΓ₁ HΓ₂]".
+    iIntros (Hop) "#He₁ #He₂ !# %vs HΓ₁ //=".
     iApply (ewp_bind [BinOpRCtx _ _]); first done.
-    iApply (ewp_mono with "[HΓ₂]").
-    { by iApply "He₂". }
-    iIntros (v) "Hv !> //=". 
-    iApply (ewp_bind [BinOpLCtx _ _]); first done.
     iApply (ewp_mono with "[HΓ₁]").
+    { by iApply "He₂". }
+    iIntros (v) "[Hv HΓ₂] !> //=". 
+    iApply (ewp_bind [BinOpLCtx _ _]); first done.
+    iApply (ewp_mono with "[HΓ₂]").
     { by iApply "He₁". }
-    iIntros (w) "Hw !> //=". 
+    iIntros (w) "[Hw HΓ₃] !> //=". 
     destruct op; inversion_clear Hop;
       iDestruct "Hv" as "(%n1 & ->)";
       iDestruct "Hw" as "(%n2 & ->)";
       ewp_pure_steps; eauto.
   Qed.
   
-  Lemma sem_typed_if Γ₁ Γ₂ e₁ e₂ e₃ ρ τ: 
-    Γ₁ ⊨ e₁ : ρ : 𝔹 -∗
-    Γ₂ ⊨ e₂ : ρ : τ -∗
-    Γ₂ ⊨ e₃ : ρ : τ -∗
-    Γ₁ ++ Γ₂ ⊨ (if: e₁ then e₂ else e₃) : ρ : τ.
+  Lemma sem_typed_if Γ₁ Γ₂ Γ₃ e₁ e₂ e₃ ρ τ: 
+    Γ₁ ⊨ e₁ : ρ : 𝔹 ⊨ Γ₂ -∗
+    Γ₂ ⊨ e₂ : ρ : τ ⊨ Γ₃ -∗
+    Γ₂ ⊨ e₃ : ρ : τ ⊨ Γ₃ -∗
+    Γ₁ ⊨ (if: e₁ then e₂ else e₃) : ρ : τ ⊨ Γ₃.
   Proof.
-    iIntros "#He₁ #He₂ #He₃ !# %vs HΓ₁₂ //=".
-    rewrite env_sem_typed_app.
-    iDestruct "HΓ₁₂" as "[HΓ₁ HΓ₂]".
-    iApply (ewp_bind [IfCtx (subst_map vs e₂) (subst_map vs e₃)])
-      ;first done.
+    iIntros "#He₁ #He₂ #He₃ !# %vs HΓ₁ //=".
+    iApply (ewp_bind [IfCtx (subst_map vs e₂) (subst_map vs e₃)]) ;first done.
     iApply (ewp_mono with "[HΓ₁]").
     { by iApply "He₁". }
-    iIntros (v) "(%b & ->)". iModIntro. simpl.
+    iIntros (v) "((%b & ->) & HΓ₃) !> //=".
     destruct b; ewp_pure_steps.
     - by iApply "He₂".
     - by iApply "He₃".
   Qed.
   
   (* Type abstraction and application *)
-  Lemma sem_typed_TLam Γ ρ e C : 
-    (∀ A, Γ ⊨ e : ρ : C A) -∗
-    Γ ⊨ (Λ: e) : ⟨⟩ : (∀: A , ρ , C A)%T.
+  Lemma sem_typed_TLam Γ₁ Γ₂ ρ e C : 
+    (∀ A, Γ₁ ⊨ e : ρ : C A ⊨ []) -∗
+    Γ₁ ++ Γ₂ ⊨ (Λ: e) : ⟨⟩ : (∀: A , ρ , C A)%T ⊨ Γ₂.
   Proof.
-    iIntros "#Hv !# %vs HΓ //=".
-    ewp_pure_steps. iIntros "%A". ewp_pure_steps.
-    by iApply "Hv".
+    iIntros "#He !# %vs HΓ₁₂ //=".
+    rewrite env_sem_typed_app.
+    iDestruct "HΓ₁₂" as "[HΓ₁ HΓ₂]".
+    ewp_pure_steps. iIntros "{$HΓ₂} %A //=". ewp_pure_steps.
+    iApply (ewp_mono with "[He HΓ₁]").
+    { by iApply "He". }
+    iIntros (w) "[HC _] !> {$HC}".
   Qed.
 
-  Lemma sem_typed_TApp Γ e ρ τ C : 
-    Γ ⊨ e : ρ : (∀: α , ρ , C α) -∗
-    Γ ⊨ e <_> : ρ : C τ. 
+  Lemma sem_typed_TApp Γ₁ Γ₂ e ρ τ C : 
+    Γ₁ ⊨ e : ρ : (∀: α , ρ , C α) ⊨ Γ₂ -∗
+    Γ₁ ⊨ e <_> : ρ : C τ ⊨ Γ₂. 
   Proof.
-    iIntros "#Hv !# %vs HΓ //=".
+    iIntros "#He !# %vs HΓ₁ //=".
     iApply (ewp_bind [AppLCtx _]); first done.
-    iApply (ewp_mono with "[HΓ]").
-    { by iApply "Hv". }
-    iIntros "%w Hw !> //=".
+    iApply (ewp_mono with "[HΓ₁]").
+    { by iApply "He". }
+    iIntros "%w [Hw HΓ₂] !> //=".
+    iApply (ewp_frame_r with "Hw HΓ₂").
   Qed.
 
   (* Existential type packing and unpacking *)
-  Lemma sem_typed_pack Γ ρ e C τ :
-    Γ ⊨ e : ρ : C τ -∗
-    Γ ⊨ (pack: e) : ρ : (∃: α, C α)%T. 
+  Lemma sem_typed_pack Γ₁ Γ₂ ρ e C τ :
+    Γ₁ ⊨ e : ρ : C τ ⊨ Γ₂ -∗
+    Γ₁ ⊨ (pack: e) : ρ : (∃: α, C α) ⊨ Γ₂. 
   Proof.
-    iIntros "#He %vs !# HΓ //=".
+    iIntros "#He %vs !# HΓ₁ //=".
     iApply (ewp_bind [AppRCtx _]); first done.
-    iApply (ewp_mono with "[HΓ]"); [by iApply "He"|].
-    iIntros (v) "Hτv !> //=".
+    iApply (ewp_mono with "[HΓ₁]"); [by iApply "He"|].
+    iIntros (v) "[Hτv HΓ₂] !> //=".
     unfold exist_pack. ewp_pure_steps.
-    by iExists τ. 
+    iFrame. by iExists τ. 
   Qed.
 
-  Lemma sem_typed_unpack Γ₁ Γ₂ x ρ e₁ e₂ κ C :
-    x ∉ env_dom Γ₂ →
-    Γ₁ ⊨ e₁ : ρ : (∃: α, C α) -∗
-    (∀ τ, (x, C τ) :: Γ₂ ⊨ e₂ : ρ : κ) -∗
-    Γ₁ ++ Γ₂ ⊨ (unpack: x := e₁ in e₂) : ρ : κ.
+  Lemma sem_typed_unpack Γ₁ Γ₂ Γ₃ x ρ e₁ e₂ κ C :
+    x ∉ env_dom Γ₂ → x ∉ env_dom Γ₃ →
+    Γ₁ ⊨ e₁ : ρ : (∃: α, C α) ⊨ Γ₂ -∗
+    (∀ τ, (x, C τ) :: Γ₂ ⊨ e₂ : ρ : κ ⊨ Γ₃) -∗
+    Γ₁ ⊨ (unpack: x := e₁ in e₂) : ρ : κ ⊨ Γ₃.
   Proof.
-    iIntros (Hnotin) "#He₁ #He₂ %vs !# HΓ₁₂ //=".
-    rewrite env_sem_typed_app.
-    iDestruct "HΓ₁₂" as "[HΓ₁ HΓ₂]".
+    iIntros (??) "#He₁ #He₂ %vs !# HΓ₁ //=".
     iApply (ewp_bind [AppRCtx _]); first done.
     iApply (ewp_mono with "[HΓ₁]"); [by iApply "He₁"|].
-    iIntros (w) "(%τ & Hτw) !> //=". unfold exist_unpack.
+    iIntros (w) "[(%τ & Hτw) HΓ₂] !> //=". unfold exist_unpack.
     ewp_pure_steps. rewrite -subst_map_insert.
-    iApply "He₂". simpl. iSplitL "Hτw".
-    { iExists w. iFrame. iPureIntro. by rewrite lookup_insert. }
-    by iApply env_sem_typed_insert.
+    iApply (ewp_mono with "[Hτw HΓ₂]").
+    - iApply "He₂". simpl. iSplitL "Hτw".
+      { iExists w. iFrame. iPureIntro. by rewrite lookup_insert. }
+      by iApply env_sem_typed_insert.
+    - iIntros (u) "[Hκ HΓ₃] !> {$Hκ}".
+      by iApply env_sem_typed_delete.
   Qed.
 
   (* Recursive type rules *)
-  Lemma sem_typed_fold Γ e ρ C `{NonExpansive C}:
-    Γ ⊨ e : ρ : (C (μ: α, C α)) -∗
-    Γ ⊨ (fold: e) : ρ : (μ: α, C α).
+  Lemma sem_typed_fold Γ₁ Γ₂ e ρ C `{NonExpansive C}:
+    Γ₁ ⊨ e : ρ : (C (μ: α, C α)) ⊨ Γ₂ -∗
+    Γ₁ ⊨ (fold: e) : ρ : (μ: α, C α) ⊨ Γ₂.
   Proof.
-    iIntros "#He %vs !# HΓ //=".
+    iIntros "#He %vs !# HΓ₁ //=".
     iApply (ewp_bind [AppRCtx _]); first done. 
-    iApply (ewp_mono with "[HΓ]"); [by iApply "He"|].
-    iIntros "%w HC !> //=". 
+    iApply (ewp_mono with "[HΓ₁]"); [by iApply "He"|].
+    iIntros "%w [HC HΓ₂] !> //=". 
     unfold rec_fold. ewp_pure_steps.
-    by iApply sem_ty_rec_unfold. 
+    iFrame. by iApply sem_ty_rec_unfold. 
   Qed.
 
-  Lemma sem_typed_unfold Γ e ρ C `{NonExpansive C}:
-    Γ ⊨ e : ρ : (μ: α, C α) -∗
-    Γ ⊨ (unfold: e) : ρ : (C (μ: α, C α)).
+  Lemma sem_typed_unfold Γ₁ Γ₂ e ρ C `{NonExpansive C}:
+    Γ₁ ⊨ e : ρ : (μ: α, C α) ⊨ Γ₂ -∗
+    Γ₁ ⊨ (unfold: e) : ρ : (C (μ: α, C α)) ⊨ Γ₂.
   Proof.
-    iIntros "#He %vs !# HΓ //=".
+    iIntros "#He %vs !# HΓ₁ //=".
     iApply (ewp_bind [AppRCtx _]); first done. 
-    iApply (ewp_mono with "[HΓ]"); [by iApply "He"|].
-    iIntros "%w Hμ !> //=". 
+    iApply (ewp_mono with "[HΓ₁]"); [by iApply "He"|].
+    iIntros "%w [Hμ HΓ₂] !> //=". 
     rewrite sem_ty_rec_unfold. 
-    unfold rec_unfold. by ewp_pure_steps.
+    unfold rec_unfold. ewp_pure_steps. iFrame.
   Qed.
 
   (* List type rules *)
   Lemma sem_typed_nil Γ τ: 
-    ⊢ Γ ⊨ NIL : ⟨⟩ : List τ.
+    ⊢ Γ ⊨ NIL : ⟨⟩ : List τ ⊨ Γ.
   Proof.
     iIntros "!# %vs HΓ //=". 
     ewp_pure_steps. unfold sem_ty_list.
-    rewrite sem_ty_rec_unfold. iNext. unfold ListF.
-    iExists (#()). by iLeft.
+    rewrite sem_ty_rec_unfold. iIntros "{$HΓ} !>".
+    unfold ListF. iExists #(). by iLeft.
   Qed.
   
-  Lemma sem_typed_cons Γ₁ Γ₂ e₁ e₂ ρ τ: 
-    Γ₁ ⊨ e₁ : ρ : τ -∗
-    Γ₂ ⊨ e₂ : ρ : List τ -∗
-    Γ₁ ++ Γ₂ ⊨ CONS e₁ e₂ : ρ : List τ.
+  Lemma sem_typed_cons Γ₁ Γ₂ Γ₃ e₁ e₂ ρ τ: 
+    Γ₂ ⊨ e₁ : ρ : τ ⊨ Γ₃-∗
+    Γ₁ ⊨ e₂ : ρ : List τ ⊨ Γ₂-∗
+    Γ₁ ⊨ CONS e₁ e₂ : ρ : List τ ⊨ Γ₃.
   Proof.
-    iIntros "#He₁ #He₂ !# %vs HΓ₁₂ //=". 
-    rewrite env_sem_typed_app.
-    iDestruct "HΓ₁₂" as "(HΓ₁ & HΓ₂)".
+    iIntros "#He₁ #He₂ !# %vs HΓ₁ //=". 
     iApply (ewp_bind [InjRCtx; PairRCtx _]); first done.
-    iApply (ewp_mono with "[HΓ₂]").
+    iApply (ewp_mono with "[HΓ₁]").
     { by iApply "He₂". }
-    iIntros (l) "Hl !> //=".
+    iIntros (l) "[Hl HΓ₂] !> //=".
     iApply (ewp_bind [InjRCtx; PairLCtx _]); first done.
-    iApply (ewp_mono with "[HΓ₁]"); [by iApply "He₁"|].
-    iIntros (x) "Hx !> //=". ewp_pure_steps.
+    iApply (ewp_mono with "[HΓ₂]"); [by iApply "He₁"|].
+    iIntros (x) "[Hx HΓ₃] !> //=". ewp_pure_steps.
     unfold sem_ty_list. rewrite !sem_ty_rec_unfold.
-    iNext. iExists (x,l)%V. iRight. iSplit; first done.
+    iIntros "{$HΓ₃} !>". iExists (x,l)%V. iRight. iSplit; first done.
     iExists x, l. iFrame; iSplit; first done.
     by rewrite sem_ty_rec_unfold. 
   Qed.
   
-  Lemma sem_typed_list_match Γ₁ Γ₂ x xs e₁ e₂ e₃ ρ τ κ :
-    x ∉ (env_dom Γ₂) ->
-    xs ∉ (env_dom Γ₂) ->
+  Lemma sem_typed_list_match Γ₁ Γ₂ Γ₃ x xs e₁ e₂ e₃ ρ τ κ :
+    x ∉ (env_dom Γ₂) -> xs ∉ (env_dom Γ₂) ->
+    x ∉ (env_dom Γ₃) -> xs ∉ (env_dom Γ₃) ->
     x ≠ xs ->
-    Γ₁ ⊨ e₁ : ρ : List τ -∗
-    Γ₂ ⊨ e₂ : ρ : κ -∗
-    ((x, τ) :: (xs, (List τ)%T) :: Γ₂) ⊨ e₃ : ρ : κ -∗
-    Γ₁ ++ Γ₂ ⊨ list-match: e₁ with 
-                    CONS x => xs => e₃ 
-                  | NIL => e₂
-                end : ρ : κ.
+    Γ₁ ⊨ e₁ : ρ : List τ ⊨ Γ₂ -∗
+    Γ₂ ⊨ e₂ : ρ : κ ⊨ Γ₃ -∗
+    (x, τ) :: (xs, List τ) :: Γ₂ ⊨ e₃ : ρ : κ ⊨ Γ₃ -∗
+    Γ₁ ⊨ list-match: e₁ with 
+            CONS x => xs => e₃ 
+          | NIL => e₂
+         end : ρ : κ ⊨ Γ₃.
   Proof.
-    iIntros (Hx Hxs Hneq) "#He₁ #He₂ #He₃ !# %vs HΓ₁₂ //=".
-    rewrite env_sem_typed_app.
-    iDestruct "HΓ₁₂" as "(HΓ₁ & HΓ₂)". 
+    iIntros (?????) "#He₁ #He₂ #He₃ !# %vs HΓ₁ //=".
     iApply (ewp_bind [CaseCtx _ _]); first done.
     iApply (ewp_mono with "[HΓ₁]"); [by iApply sem_typed_unfold|simpl].
-    unfold sem_ty_list. iIntros (v₁) "Hl !>". ewp_pure_steps.
-    iDestruct "Hl" as "(%v' & [(-> & Hunit)|(-> & (%w₁ & %w₂ & -> & Hτ & Hμ))])"; ewp_pure_steps.
+    unfold sem_ty_list. iIntros (v₁) "[Hl HΓ₂] !>". ewp_pure_steps.
+    iDestruct "Hl" as "(%v' & [[-> ->]|(-> & (%w₁ & %w₂ & -> & Hτ & Hμ))])"; 
+    ewp_pure_steps.
     { iApply ("He₂" with "[$HΓ₂]"). }
     rewrite lookup_delete. simpl.
     rewrite decide_False; [|by intros [_ []]].
@@ -385,189 +395,198 @@ Section compatibility.
     rewrite insert_delete_insert. rewrite subst_map_insert.
     rewrite subst_subst_ne; [|congruence]. rewrite delete_commute.
     rewrite -subst_map_insert -delete_insert_ne; try congruence.
-    rewrite -subst_map_insert. iApply "He₃". simpl.
-    iSplitL "Hτ".
-    { iExists w₁. iFrame. by rewrite lookup_insert. }
-    iSplitL "Hμ".
-    + iExists w₂. unfold sem_ty_list. iSplitR; [|done].
-      rewrite lookup_insert_ne; [|congruence].  
-      by rewrite lookup_insert. 
-    + iApply env_sem_typed_insert; first done.
-      by iApply env_sem_typed_insert; first done.
+    rewrite -subst_map_insert. 
+    iApply (ewp_mono with "[Hτ Hμ HΓ₂]").
+    - iApply "He₃". simpl.
+      iSplitL "Hτ".
+      { iExists w₁. iFrame. by rewrite lookup_insert. }
+      iSplitL "Hμ".
+      + iExists w₂. unfold sem_ty_list. iSplitR; [|done].
+        rewrite lookup_insert_ne; [|congruence].  
+        by rewrite lookup_insert. 
+      + iApply env_sem_typed_insert; first done.
+        by iApply env_sem_typed_insert; first done.
+    - iIntros (u) "[Hκ HΓ₃] !> {$Hκ}".
+      iApply (env_sem_typed_delete _ _ xs w₂); first done.
+      iApply (env_sem_typed_delete _ _ x w₁); done.
   Qed.
 
 
   (* Reference rules *)
   
-  (* The references that we implement here are always copyable, 
-     so we have ∀ τ, copy_ty (Ref τ).
-     This allows us to treat references in a non sub-structural way.
-     Since we do not have `free` in our language
-     we do not have use-after-free and double-free problems
-     and so making them persistent will be too restrictive.
-     This is why the `load` does not return the reference back
-     and we can always `load` from the same reference more than once.
-  
-     The down side of this is that we cannot store
-     non-persistent functions like continuations.
-  *)
-     
-  Lemma sem_typed_alloc Γ e ρ τ: 
-    copy_ty τ →
-    Γ ⊨ e : ρ : τ -∗
-    Γ ⊨ ref e : ρ : Ref τ.
+  Lemma sem_typed_alloc Γ₁ Γ₂ e ρ τ: 
+    Γ₁ ⊨ e : ρ : τ ⊨ Γ₂ -∗
+    Γ₁ ⊨ ref e : ρ : Ref τ ⊨ Γ₂.
   Proof.
-    iIntros (Hcpyτ) "#He !# %vs HΓ //=".
+    iIntros "#He !# %vs HΓ₁ //=".
     iApply (ewp_bind [AllocCtx]); first done. simpl.
-    iApply (ewp_mono with "[HΓ]").
-    { by iApply "He". }
-    iIntros (v) "Hτ". iModIntro.
-    iApply ewp_alloc. iIntros "!> %l Hl".
-    iMod (inv_alloc (tyN.@l) _
-         (∃ w, l ↦ w ∗ τ w)%I with "[Hl Hτ]") as "#Hinv".
-    { iExists v. by iFrame. }
-    iModIntro. iExists l. do 2 (iSplit; try done).
-    by iApply copy_pers.
-  Qed.
-  
-  Lemma sem_typed_load Γ e ρ τ: 
-    Γ ⊨ e : ρ : Ref τ -∗
-    Γ ⊨ !e : ρ : τ.
-  Proof.
-    iIntros "#He !# %vs HΓ //". simpl.
-    iApply (ewp_bind [LoadCtx]); first done. simpl.
-    iApply (ewp_mono with "[HΓ]").
-    { by iApply "He". }
-    iIntros (v) "(%l & -> & #Hcpy & #Hinv)". iModIntro.
-    iApply (ewp_atomic _ (⊤ ∖ ↑tyN.@l)).
-    iMod (inv_acc _ (tyN.@l) with "Hinv") as "[(%w & >Hl & HA) Hclose]"; 
-      first done.
-    iModIntro. iApply (ewp_load with "Hl").
-    iNext. 
-    iDestruct ("Hcpy" with "HA") as "#Hτ".
-    iIntros "Hl !>". simpl.
-    iMod ("Hclose" with "[Hl]"); last done.
-    iExists w. by iFrame.
-  Qed.
-  
-  Lemma sem_typed_store Γ₁ Γ₂ e₁ e₂ ρ τ: 
-    Γ₁ ⊨ e₁ : ρ : Ref τ -∗
-    Γ₂ ⊨ e₂ : ρ : τ -∗
-    Γ₁ ++ Γ₂ ⊨ (e₁ <- e₂) : ρ : ().
-  Proof.
-    iIntros "#He₁ #He₂ !# %vs HΓ₁₂ //=".
-    rewrite !env_sem_typed_app.
-    iDestruct "HΓ₁₂" as "(HΓ₁ & HΓ₂)". 
-    iApply (ewp_bind [StoreRCtx _]); first done. simpl.
-    iApply (ewp_mono with "[HΓ₂]").
-    { by iApply "He₂". }
-    iIntros (v) "Hτ". iModIntro.
-    iApply (ewp_bind [StoreLCtx _]); first done. simpl.
     iApply (ewp_mono with "[HΓ₁]").
-    { by iApply "He₁". }
-    iIntros (w) "(%l & -> & #Hcpy & #Hinv)". iModIntro.
-    iApply (ewp_atomic _ (⊤ ∖ ↑tyN.@l)).
-    iMod (inv_acc _ (tyN.@l) with "Hinv") as "[(%w & >Hl & HA) Hclose]"; 
-      first done.
-    iModIntro. iApply (ewp_store with "Hl").
-    iIntros "!> Hl !>". 
-    iMod ("Hclose" with "[Hl Hτ]"); last done.
-    iExists v. by iFrame. 
+    { by iApply "He". }
+    iIntros (v) "[Hτ HΓ₂] !>".
+    iApply ewp_alloc. iIntros "!> %l Hl !> {$HΓ₂}".
+    iExists l. iSplit; first done. iExists v. iFrame.
+  Qed.
+  
+  Lemma sem_typed_load Γ x ρ τ: 
+    ⊢ ((x, Ref τ) :: Γ ⊨ !x : ρ : τ ⊨ (x, Ref Moved) :: Γ).
+  Proof.
+    iIntros "%vs !# //= [(%v & -> & (%l & -> & (%w & Hl & Hτ))) HΓ] //=". 
+    iApply (ewp_load with "Hl").
+    iIntros "!> Hl !> {$Hτ} {$HΓ}". iExists #l.
+    iSplitR; first done. iExists l. iSplitR; first done.
+    iExists w. iFrame.
+  Qed.
+  
+  Lemma sem_typed_load_copy Γ x ρ τ: 
+    copy_ty τ →
+    ⊢ ((x, Ref τ) :: Γ ⊨ !x : ρ : τ ⊨ (x, Ref τ) :: Γ).
+  Proof.
+    iIntros (Hcpy) "%vs !# //= [(%v & -> & (%l & -> & (%w & Hl & Hτ))) HΓ] //=". 
+    iApply (ewp_load with "Hl").
+    unfold copy_ty, Persistent in Hcpy.
+    iDestruct (Hcpy w with "Hτ") as "#Hτ'". 
+    iIntros "!> Hl !> {$Hτ} {$HΓ}". iExists #l.
+    iSplitR; first done. iExists l. iSplitR; first done.
+    iExists w. iFrame. iApply "Hτ'".
+  Qed.
+
+  Lemma sem_typed_store Γ₁ Γ₂ x e ρ τ κ: 
+    Γ₁ ⊨ e : ρ : κ ⊨ Γ₂ -∗
+    (x, Ref τ) :: Γ₁ ⊨ (x <- e) : ρ : () ⊨ (x, Ref κ) :: Γ₂.
+  Proof.
+    iIntros "#He !# %vs //= [(%v & -> & (%l & -> & (%u & Hl & Hτ))) HΓ₁] //=".
+    iApply (ewp_bind [StoreRCtx _]); first done. simpl.
+    iApply (ewp_mono with "[HΓ₁]").
+    { by iApply "He". }
+    iIntros (w) "[Hκ HΓ₂] !>".
+    iApply (ewp_store with "Hl"). iIntros "!> Hl !> {$HΓ₂}". 
+    iSplitR; first done. iExists #l. iSplitR; first done.
+    iExists l. iSplitR; first done. iExists w. iFrame.
   Qed.
   
   (* Effect handling rules *)
   
-  Lemma sem_typed_do Γ e ι κ: 
-    Γ ⊨ e : (ι ⇒ κ) : ι -∗
-    Γ ⊨ (do: e) : (ι ⇒ κ) : κ.
+  Lemma sem_typed_do Γ₁ Γ₂ e ι κ: 
+    Γ₁ ⊨ e : (ι ⇒ κ) : ι ⊨ Γ₂ -∗
+    Γ₁ ⊨ (do: e) : (ι ⇒ κ) : κ ⊨ Γ₂.
   Proof.
-    iIntros "#He !# %vs HΓ //=". 
+    iIntros "#He !# %vs HΓ₁ //=". 
     iApply (ewp_bind [DoCtx OS]); first done.
-    iApply (ewp_mono with "[HΓ]").
+    iApply (ewp_mono with "[HΓ₁]").
     { by iApply "He". }
-    iIntros (v) "Hι". iModIntro. simpl.
+    iIntros (v) "[Hι HΓ₂] !> //=".
     iApply ewp_do_os. rewrite upcl_sem_row_eff.
     iExists v. eauto with iFrame.
   Qed.
   
   
-  Lemma sem_typed_shallow_try Γ₁ Γ₂ e h r ι κ τ τ': 
+  (* Limitation: 
+     In the typing rule for the effect branch, the continuation
+     has the additional information that when called it returns
+     a value of type τ' and that env_sem_typed Γ₂ vs holds.
+     But because the type signature of the handler is simply:
+     ι ⊸ (k -{ ρ }-∘ τ' -{ ρ }-∘ τ 
+     this extra env_sem_typed Γ₂ vs is ignored and cannot be
+     used inside the handler, so we have some loss of information.
+   *)
+  Lemma sem_typed_shallow_try Γ₁ Γ₂ Γ₃ Γ' w k x e h r ι κ τ τ': 
+    x ∉ env_dom Γ₂ → x ∉ env_dom Γ' → x ∉ env_dom Γ₃ →
+    w ∉ env_dom Γ' → w ∉ env_dom Γ' → k ∉ env_dom Γ' → k ∉ env_dom Γ' → 
+    w ∉ env_dom Γ₃ → w ∉ env_dom Γ₃ → k ∉ env_dom Γ₃ → k ∉ env_dom Γ₃ → w ≠ k →
     let ρ := (ι ⇒ κ)%R in
-    Γ₁ ⊨ e : ρ : τ' -∗
-    Γ₂ ⊨ h : ⟨⟩ : (ι ⊸ (κ -{ ρ }-∘ τ') -{ ρ }-∘ τ) -∗
-    Γ₂ ⊨ r : ⟨⟩ : (τ' -{ ρ }-∘ τ) -∗
-    Γ₁ ++ Γ₂ ⊨ (TryWith e h r) : (ι ⇒ κ) : τ.
+    Γ₁ ⊨ e : ρ : τ' ⊨ Γ₂ -∗
+    (w, ι) :: (k, κ -{ ρ }-∘ τ') :: Γ' ⊨ h w k : ρ : τ ⊨ Γ₃ -∗
+    (x, τ') :: Γ₂ ++ Γ' ⊨ r x : ρ : τ ⊨ Γ₃ -∗
+    Γ₁ ++ Γ' ⊨ (TryWith e (λ: w k, h w k) (λ: x, r x)) : (ι ⇒ κ) : τ ⊨ Γ₃.
   Proof.
-    iIntros "%ρ #He #Hh #Hr !# %vs HΓ₁₂ //=".
-    rewrite !env_sem_typed_app.
-    iDestruct "HΓ₁₂" as "(HΓ₁ & HΓ₂)". ewp_pure_steps.
-    iApply (ewp_try_with with "[HΓ₁] [HΓ₂]").
+    iIntros (????????????) "%ρ #He #Hh #Hr !# %vs HΓ₁' //=".
+    rewrite env_sem_typed_app.
+    iDestruct "HΓ₁'" as "[HΓ₁ HΓ']".
+    ewp_pure_steps.
+    iApply (ewp_try_with with "[HΓ₁]").
     { by iApply "He". }
-    iSplit; [|iSplit; iIntros (v k)];
-    last (iIntros "HFalse"; by rewrite upcl_bottom).
-    - iIntros (v) "Hv //=".
-      iApply (ewp_bind [AppLCtx v]); first done.
-      ewp_bottom.
-      iApply (ewp_mono with "[HΓ₂]"); [by iApply "Hr"|].
-      iIntros (w) "Hw". iModIntro. simpl.
-      by iApply "Hw".
+    iSplit; [|iSplit; iIntros (v c)];
+    last (iIntros "?"; by rewrite upcl_bottom).
+    - iIntros (v) "[Hv HΓ₂] //=". ewp_pure_steps.
+      rewrite -subst_map_insert.
+      iApply (ewp_mono with "[HΓ₂ HΓ' Hv]"). 
+      + iApply "Hr". simpl. iSplitL "Hv".
+        { iExists v. iIntros "{$Hv} !%". apply lookup_insert. }
+        rewrite env_sem_typed_app. iFrame. 
+        iSplitL "HΓ₂"; by iApply env_sem_typed_insert.
+      + iIntros (u) "[Hw HΓ₃] !> //=".
+        iFrame. by iApply (env_sem_typed_delete _ _ x v).
     - rewrite upcl_sem_row_eff.
-      iIntros "(%a & -> & Ha & Hκb)".
-      iApply (ewp_bind [AppLCtx k; AppLCtx a]); first done.
-      ewp_bottom.
-      iApply (ewp_mono with "[HΓ₂]").
-      { by iApply "Hh". }
-      iIntros (h') "Hh'". iModIntro. simpl. 
-      iApply (ewp_bind [AppLCtx k]); first done. 
-      iApply (ewp_mono with "[Hh' Ha]").
-      { ewp_bottom. by iApply "Hh'". }
-      iIntros (ha) "Hha". iModIntro. simpl.
-      iApply "Hha". iIntros (w) "Hw".
-      by iApply "Hκb".
+      iIntros "(%a & -> & Ha & Hκb) //=". ewp_pure_steps. 
+      rewrite decide_True; [|split; first done; by injection].
+      rewrite subst_subst_ne; last done.
+      rewrite -subst_map_insert -delete_insert_ne; last done.
+      rewrite -subst_map_insert.
+      iApply (ewp_mono with "[HΓ' Hκb Ha]").
+      + iApply "Hh". simpl. iSplitL "Ha".
+        { iExists a. iIntros "{$Ha} !%". apply lookup_insert. }
+        iSplitL "Hκb". 
+        { iExists c. iSplitR; [iPureIntro; rewrite lookup_insert_ne; last done; apply lookup_insert|].
+          iIntros (b) "Hb".  iApply (ewp_mono with "[Hb Hκb]"); [by iApply "Hκb"|].
+          iIntros (?) "[? _] !> //=". }
+        iApply env_sem_typed_insert; first done.
+        by iApply env_sem_typed_insert; first done.
+      + iIntros (u) "[Hu HΓ₃] !> {$Hu}".
+        iApply (env_sem_typed_delete _ _ k c); first done.
+        by iApply (env_sem_typed_delete _ _ w a).
   Qed.
   
-  Lemma sem_typed_deep_try Γ₁ Γ₂ Γ₃ e h r ρ' ι κ τ τ': 
+  Lemma sem_typed_deep_try Γ₁ Γ' Γ₂ Γ₃ e x w k h r ρ' ι κ τ τ':
+    x ∉ env_dom Γ₂ → x ∉ env_dom Γ' → x ∉ env_dom Γ₃ →
+    w ∉ env_dom Γ' → w ∉ env_dom Γ₃ →
+    k ∉ env_dom Γ' → k ∉ env_dom Γ₃ → w ≠ k → copy_env Γ' →
     let ρ := (ι ⇒ κ)%R in
-    Γ₁ ⊨ e : ρ : τ -∗
-    Γ₂ ⊨ h : ⟨⟩ : (ι → (κ -{ ρ' }-∘ τ') -{ ρ' }-∘ τ') -∗
-    Γ₃ ⊨ r : ⟨⟩ : (τ -{ ρ' }-∘ τ') -∗
-    Γ₁ ++ Γ₂ ++ Γ₃ ⊨ (deep-try: e with effect h | return r end) : ρ' : τ'.
+    Γ₁ ⊨ e : ρ : τ ⊨ Γ₂ -∗
+    (w, ι) :: (k, κ -{ ρ' }-∘ τ') :: Γ' ⊨ h w k : ρ' : τ' ⊨ Γ₃ -∗
+    (x, τ) :: Γ₂ ++ Γ' ⊨ r x : ρ' : τ' ⊨ Γ₃ -∗
+    Γ₁ ++ Γ' ⊨ (deep-try: e with effect (λ: w k, h w k) | return (λ: x, r x) end) : ρ' : τ' ⊨ Γ₃.
   Proof.
-    iIntros "%ρ #He #Hh #Hr !# %vs HΓ₁₂₃ //=".
-    rewrite !env_sem_typed_app. 
-    iDestruct "HΓ₁₂₃" as "(HΓ₁ & HΓ₂ & HΓ₃)". ewp_pure_steps.
-    set ctx_r := AppRCtx (deep_try_with (λ: <>, subst_map vs e) 
-                                        (subst_map vs h))%E.
-    iApply (ewp_bind [ctx_r]); first done.
-    ewp_bottom.
-    iApply (ewp_mono with "[HΓ₃]").
-    { by iApply "Hr". }
-    iIntros (r') "Hr'". iModIntro. simpl.
+    iIntros (???????? Hcpy) "%ρ #He #Hh #Hr !# %vs HΓ₁' //=".
+    rewrite env_sem_typed_app.
+    iDestruct "HΓ₁'" as "[HΓ₁ HΓ']".
+    unfold copy_env, Persistent in Hcpy.
+    iDestruct (Hcpy vs with "HΓ'") as "#HΓ".
     ewp_pure_steps.
-    set ctx_h := [
-      AppLCtx r';
-      AppRCtx (deep_try_with (λ: <>, subst_map vs e))%E].
-    iApply (ewp_bind ctx_h); first done.
-    ewp_bottom.
-    iApply (ewp_mono with "[HΓ₂]"); [by iApply "Hh"|].
-    iIntros (h') "#Hh'". iModIntro. simpl. ewp_pure_steps.
     iApply (ewp_deep_try_with with "[HΓ₁]").
     { by iApply "He". }
-    iLöb as "IH".
-    rewrite !deep_handler_unfold.
-    iSplit; [|iSplit; iIntros (v k)];
-    last (iIntros "HFalse"; by rewrite upcl_bottom).
-    - iIntros (v) "Hv //=".
-      by iApply "Hr'".
+    iLöb as "IH". rewrite !deep_handler_unfold.
+    iSplit; [|iSplit; iIntros (v c)];
+    last (iIntros "?"; by rewrite upcl_bottom).
+    - iIntros (v) "[Hv HΓ₂] //=". ewp_pure_steps.
+      rewrite -subst_map_insert. iApply (ewp_mono with "[Hv HΓ₂ HΓ']").
+      + iApply "Hr". simpl. iSplitL "Hv".
+        iExists v. iIntros "{$Hv} !%". apply lookup_insert.
+        rewrite env_sem_typed_app. iSplitL "HΓ₂".
+        by iApply env_sem_typed_insert.
+        by iApply env_sem_typed_insert.
+      + iIntros (?) "[Hτ' HΓ₃] !> {$Hτ'}".
+        by iApply (env_sem_typed_delete _ _ x v).
     - rewrite upcl_sem_row_eff.
-      iIntros "(%a & -> & Ha & Hκb)".
-      iApply (ewp_bind [AppLCtx k]); first done. 
-      ewp_bottom. simpl. 
-      iApply (ewp_mono with "[Ha]"); [by iApply "Hh'"|].
-      iIntros (ha) "Hha !>". iApply "Hha".
-      iIntros (w) "Hw". iApply ("Hκb" with "Hw"). 
-      iNext. rewrite !deep_handler_unfold. 
-      iApply ("IH" with "Hr'").
+      iIntros "(%a & -> & Ha & Hκb)". ewp_pure_steps.
+      rewrite decide_True; [|split; first done; by injection].
+      rewrite subst_subst_ne; last done.
+      rewrite -subst_map_insert -delete_insert_ne; last done.
+      rewrite -subst_map_insert.
+      iApply (ewp_mono with "[Ha HΓ' Hκb]").
+      + iApply "Hh". simpl.
+        iSplitL "Ha"; [iExists a; iIntros "{$Ha} !%"; apply lookup_insert|].
+        iSplitL "Hκb".
+        { iExists c. iSplitR; [iPureIntro; rewrite lookup_insert_ne; last done; apply lookup_insert|].
+          iIntros (b) "Hb". iApply (ewp_mono with "[Hb Hκb]"). 
+          { iApply ("Hκb" with "Hb"). iNext.
+            rewrite !deep_handler_unfold. 
+            iApply "IH". iApply "HΓ". }
+          iIntros (v) "[Hτ' HΓ₃] !> {$Hτ'}". }
+        iApply env_sem_typed_insert; first done.
+        by iApply env_sem_typed_insert.
+      + iIntros (u) "[Hτ' HΓ₃] !> {$Hτ'}".
+        iApply (env_sem_typed_delete _ _ k c); first done.
+        by iApply (env_sem_typed_delete _ _ w a).
     Qed.
 
 End compatibility.
